MIPRE.lean
@@ -592,6 +592,7 @@ import MIPRE.Foundations.Pipeline.Oracularization
 import MIPRE.Foundations.Pipeline.Repetition
 import MIPRE.Foundations.Repeat.Bits
 import MIPRE.Foundations.Repeat.DecLoop
+import MIPRE.Foundations.Repeat.DecMain
 import MIPRE.Foundations.Repeat.MapLoop
 import MIPRE.Foundations.Repeat.Prims
 import MIPRE.Foundations.Repeat.RepSampler
